theories/MetaTheory/SubjectReduction.v
@@ -1,0 +1,155 @@
+From Metaprog Require Import Prelude.
+From Metaprog Require Export MetaTheory.Typing.
+
+(** This module proves the subject reduction (aka preservation) lemma:
+    reducing a well-typed term doesn't change its type. *)
+
+(***********************************************************************)
+(** * Context conversion. *)
+(***********************************************************************)
+
+Inductive conv_context (Σ : evar_map) : forall {s}, context ∅ s -> context ∅ s -> Prop :=
+| conv_context_nil : conv_context Σ CNil CNil
+| conv_context_cons {s} Γ Γ' x (ty ty' : term s) :
+    conv_context Σ Γ Γ' ->
+    Σ ⊢ ty ≡ ty' ->
+    conv_context Σ (CCons Γ x ty) (CCons Γ' x ty').
+
+Derive Signature for conv_context.
+
+#[export] Instance conv_context_Reflexive s Σ : Reflexive (@conv_context Σ s).
+Proof. intros Γ. induction Γ ; now constructor. Qed.
+
+#[export] Instance conv_context_Symmetric s Σ : Symmetric (@conv_context Σ s).
+Proof. intros Γ Γ' H. induction H ; now constructor. Qed.
+
+Lemma conv_context_lookup {s} Σ Γ Γ' (i : index s) :
+  conv_context Σ Γ Γ' ->
+  Σ ⊢ lookup_context i Γ ≡ lookup_context i Γ'.
+Proof.
+intros H. induction H.
+- reflexivity.
+- depelim i ; simp lookup_context.
+  + unfold wk. now apply conv_rename.
+  + unfold wk. now apply conv_rename.
+Qed.
+
+(*Lemma aux {s} Σ Γ Γ' (i : index s) :
+  conv_context Σ Γ Γ' ->
+  typing_context Σ Γ' ->
+  Σ ;; Γ' ⊢ lookup_context i Γ : TType.
+Proof.
+intros H. induction H ; intros H' ; depelim i ; simp lookup_context ; simpl_subst.
+- change TType with (rename (@rshift s x) TType). apply typing_rename with Γ'.
+  + depelim H'. admit.
+  + apply typing_rshift.*)
+
+(*Lemma typing_conv_context {s} Σ Γ Γ' (t T : term s) :
+  Σ ;; Γ ⊢ t : T ->
+  conv_context Σ Γ Γ' ->
+  typing_context Σ Γ' ->
+  Σ ;; Γ' ⊢ t : T.
+Proof.
+intros Ht. induction Ht ; intros HΓ1 HΓ2.
+- constructor.
+- subst. apply typing_conv_type with (lookup_context i Γ').
+  + now apply typing_var.
+  + symmetry. now apply conv_context_lookup.
+  + apply H
+Admitted.*)
+
+(** Beta reduction preserves typing. *)
+Lemma typing_beta {s} Σ Γ x ty body arg args (T : term s) :
+  typing_evar_map Σ ->
+  typing_context Σ Γ ->
+  Σ ;; Γ ⊢ TApp (TLam x ty body) (arg :: args) : T ->
+  Σ ;; Γ ⊢ TApp (body[x := arg]) args : T.
+Proof.
+intros HΣ HΓ H. pose proof (HT := typing_type_ok _ _ _ _ HΣ HΓ H).
+apply typing_app_inv in H. destruct H as (f_ty & T' & H1 & H2 & H3).
+apply typing_conv_type with T' ; [|assumption..]. clear T H3 HT.
+
+apply typing_lam_inv in H1. destruct H1 as (body_ty & H1 & Hty & Hbody).
+depelim H2. assert (x0 = x) as ->. { destruct x0 ; destruct x ; reflexivity. }
+apply conv_prod_inv in H1. destruct H1 as (Ha & Hb).
+apply typing_app with (b[x := arg]). ; [|assumption].
+
+
+rewrite H1 in H0. clear f_ty H1. apply conv_prod_inv in H0. destruct H0 as (Ha & Hb).
+eapply typing_app with (b[x := arg]) ; [|assumption].
+apply typing_substitute with (CCons Γ x a).
+(*- apply typing_conv_type with body_ty ; auto.
+  apply typing_prod_inv in H. apply typing_conv_context with (CCons Γ x a).
+  + apply H.
+  + admit.
+  + constructor.
+- apply typing_scons ; simpl_subst.
+  + apply typing_conv_type with a ; auto. now symmetry.
+  + apply typing_sid.
+Qed.*)
+Admitted.
+
+(** One-step reduction preserves typing. *)
+Lemma typing_red1 {s} Σ Γ (t u T : term s) :
+  typing_evar_map Σ ->
+  typing_context Σ Γ ->
+  Σ ;; Γ ⊢ t : T ->
+  Σ ⊢ t ~>₁ u ->
+  Σ ;; Γ ⊢ u : T.
+Proof.
+intros HΣ HΓ Ht Hred. depind Hred.
+- eapply typing_beta ; eauto.
+- eapply typing_evar_expand ; eauto.
+- admit.
+- apply typing_lam_inv in Ht. destruct Ht as (body_ty & HT & Hty & Hbody).
+  apply IHHred in Hbody ; auto.
+  + apply typing_conv_type with (TProd x ty body_ty).
+    * apply typing_lam ; auto.
+    * now symmetry.
+    *
+  + constructor ; auto.
+
+(*apply typing_lam_inv in Ht. destruct Ht as (body_ty & H1 & Hty & Hbody).
+  apply IHHred in Hty ; auto. rewrite Hred in H1.
+  apply typing_conv_type with (TProd x ty' body_ty).
+  + apply typing_lam.
+    * assumption.
+    *
+
+  apply typing_lam. apply IHHred.*)
+
+
+apply HΣ in H. depelim H.  depelim Ht. apply typing_evar_entry.
+
+Admitted.
+
+(** Evar expansion preserves typing. *)
+Lemma typing_evar_expand {s} Σ Γ ev ty def (T : term s) :
+  typing_evar_map Σ ->
+  typing_context Σ Γ ->
+  Σ ;; Γ ⊢ TEvar ev : T ->
+  Σ ev = Some (mk_evar_entry ty (Some def)) ->
+  Σ ;; Γ ⊢ wk def : T.
+Proof.
+intros HΣ HΓ Hev Hentry. apply typing_conv_type with (wk ty).
+- unfold wk. apply typing_rename with CNil.
+  + apply HΣ in Hentry. depelim Hentry. assumption.
+  + intros i. depelim i.
+- apply typing_evar_inv in Hev. destruct Hev as (entry & H & HT).
+  rewrite H in Hentry. depelim Hentry. cbn in HT. now symmetry.
+- eapply typing_type_ok ; eauto.
+Qed.
+
+
+(** Changing a term to a convertible one doesn't change its type. *)
+Lemma typing_conv {s} Σ Γ (t u T : term s) :
+  Σ ;; Γ ⊢ t : T ->
+  Σ ⊢ t ≡ u ->
+  Σ ;; Γ ⊢ u : T.
+Proof. Admitted.
+
+#[export] Instance typing_conv_Proper {s} Σ Γ :
+  Proper (conv Σ ==> eq ==> iff) (@typing s Σ Γ).
+Proof.
+intros t t' Ht T T' ->. split ; intros H ; eapply typing_conv ; eauto. now symmetry.
+Qed.
